generalize ctor id to simplify equational theories

DY/Bytes/EquationalTheory.lean
@@ -3,14 +3,16 @@ import DY.Kleene
 
 namespace DY
 
-structure AttackerKnowledge [BytesCtors] where
+structure AttackerKnowledge {CtorId} [BytesCtors CtorId] where
   pred: (Bytes → Prop) → Bytes → Prop
   pred_scott_continuous: DY.Kleene.IsScottContinuous pred
 
 structure EquationalTheory where
   ctors: List BytesCtor
   attackerKnowledge:
-    [BytesCtors] → [Bytes.HasCtors ctors] →
+    {CtorId: Type} → [DecidableEq CtorId] →
+    [BytesCtors CtorId] → [Ord Bytes] →
+    [Bytes.HasCtors ctors] →
     List AttackerKnowledge
 
 -- This typeclass is useful in the following situation:
@@ -24,7 +26,7 @@ structure EquationalTheory where
 --   Bytes.HasCtors myEqThy.ctors
 -- (through the instance of HasEquationalTheory myEqThy)
 class EquationalTheory.CtorsEq (theory: semiOutParam EquationalTheory) (ctors: List BytesCtor) where
-  pf: theory.ctors = ctors
+  pf (theory ctors): theory.ctors = ctors
 
 instance: EquationalTheory.CtorsEq theory theory.ctors where
   pf := rfl
@@ -34,49 +36,91 @@ class EquationalTheories where
 
 abbrev TheoryId [EquationalTheories]: Type := Fin (EquationalTheories.theories.length)
 
-def BytesCtors.ofList (ctorsList: List BytesCtor): BytesCtors where
-  n := ctorsList.length
-  ctors i := ctorsList[i]
+structure CtorId [EquationalTheories] where
+  idThy: TheoryId
+  idCtor: Fin EquationalTheories.theories[idThy].ctors.length
+deriving DecidableEq
 
-instance [EquationalTheories]: BytesCtors := BytesCtors.ofList (EquationalTheories.theories.flatMap EquationalTheory.ctors)
+instance [EquationalTheories]: Ord CtorId where
+  compare id1 id2 :=
+    let {idThy := idThy1, idCtor := idCtor1} := id1
+    let {idThy := idThy2, idCtor := idCtor2} := id2
+    match h: compare idThy1 idThy2 with
+    | .lt => .lt
+    | .gt => .gt
+    | .eq => by
+      simp at h
+      subst h
+      exact (
+        compare idCtor1 idCtor2
+      )
 
-def computeCtorIndex (l: List EquationalTheory) (i: Nat): Nat :=
-  match l, i with
-  | [], _ => 0
-  | _, 0 => 0
-  | h::t, i+1 =>
-    h.ctors.length + computeCtorIndex t i
+instance [EquationalTheories]: Std.ReflOrd CtorId where
+  compare_self {id} := by
+    let {idThy, idCtor} := id
+    unfold compare instOrdCtorId; simp only
+    have: compare idThy idThy = .eq := by simp
+    rewrite [this]
+    simp
 
-theorem computeCtorIndex_in_bounds (l: List EquationalTheory) (i: Nat) (j: Nat) (h_i: i < l.length) (h_j: j < l[i].ctors.length):
-  computeCtorIndex l i + j < (l.flatMap EquationalTheory.ctors).length
-  := by
-    induction l generalizing i with
-    | nil => grind
-    | cons h t ih =>
-      cases i with
-      | zero =>
-        simp [computeCtorIndex]
+instance [EquationalTheories]: Std.LawfulEqOrd CtorId where
+  eq_of_compare {id1 id2} := by
+    let {idThy := idThy1, idCtor := idCtor1} := id1
+    let {idThy := idThy2, idCtor := idCtor2} := id2
+    unfold compare instOrdCtorId; simp only
+    split
+    · grind
+    · grind
+    · have : idThy1 = idThy2 := by grind
+      subst this
+      simp
+
+instance [EquationalTheories]: Std.OrientedOrd CtorId where
+  eq_swap {id1 id2} := by
+    let {idThy := idThy1, idCtor := idCtor1} := id1
+    let {idThy := idThy2, idCtor := idCtor2} := id2
+    unfold compare instOrdCtorId; simp only
+    have idThy_swap: compare idThy1 idThy2 = (compare idThy2 idThy1).swap := Std.OrientedOrd.eq_swap
+    split
+    · split <;> grind
+    · split <;> grind
+    have heq: idThy1 = idThy2 := by grind
+    subst heq
+    dsimp only
+    have idCtor_swap: compare idCtor1 idCtor2 = (compare idCtor2 idCtor1).swap := Std.OrientedOrd.eq_swap
+    split <;> grind
+
+instance [EquationalTheories]: Std.TransOrd CtorId where
+  isLE_trans := by
+    apply mkTransitive
+    · simp
+    intro id1 id2 id3
+    let {idThy := idThy1, idCtor := idCtor1} := id1
+    let {idThy := idThy2, idCtor := idCtor2} := id2
+    let {idThy := idThy3, idCtor := idCtor3} := id3
+    unfold compare instOrdCtorId; simp only
+    intro h12 h23
+    split at h12 <;> rename_i h_idThy12
+    · split at h23 <;> rename_i h_idThy23
+      · have := Std.TransCmp.lt_trans h_idThy12 h_idThy23
         grind
-      | succ i =>
-        have := ih i (by grind) (by grind)
-        simp [computeCtorIndex]
-        simp_all +arith
+      · contradiction
+      · grind
+    · contradiction
+    · split at h23 <;> rename_i h_idThy23
+      · grind
+      · contradiction
+      · have h_idThy12_eq := Std.LawfulEqOrd.eq_of_compare h_idThy12
+        have h_idThy23_eq := Std.LawfulEqOrd.eq_of_compare h_idThy23
+        subst h_idThy12_eq
+        subst h_idThy23_eq
+        dsimp only at *
+        rewrite [h_idThy12]
+        dsimp only
+        exact Std.TransCmp.lt_trans h12 h23
 
-theorem computeCtorIndex_getElem (l: List EquationalTheory) (i: Nat) (j: Nat) (h_i: i < l.length) (h_j: j < l[i].ctors.length):
-  (l.flatMap EquationalTheory.ctors)[computeCtorIndex l i + j]'(computeCtorIndex_in_bounds l i j h_i h_j) = l[i].ctors[j]
-  := by
-    induction l generalizing i with
-    | nil => grind
-    | cons h t ih =>
-      cases i with
-      | zero =>
-        simp [computeCtorIndex]
-        grind
-      | succ i =>
-        have := ih i (by grind) (by grind)
-        simp [computeCtorIndex]
-        grind
-
+instance [EquationalTheories]: BytesCtors CtorId where
+  ctors id := EquationalTheories.theories[id.idThy].ctors[id.idCtor]
 
 class HasEquationalTheory [EquationalTheories] (theory: EquationalTheory) where
   id: TheoryId
@@ -101,9 +145,9 @@ theorem HasEquationalTheory.ext
 
 def EquationalTheory.into_theory_id
   [EquationalTheories]
-  (theory: EquationalTheory)
+  {theory: EquationalTheory}
   [inst: HasEquationalTheory theory]
-  (P: (theory: EquationalTheory) → [HasEquationalTheory theory] → Sort u)
+  {P: (theory: EquationalTheory) → [HasEquationalTheory theory] → Sort u}
   (x: P EquationalTheories.theories[inst.id])
   : P theory
   := by
@@ -115,110 +159,34 @@ def EquationalTheory.into_theory_id
     apply HasEquationalTheory.ext
     simp [HasEquationalTheory.id]
 
-def EquationalTheory.toGlobalIndex [EquationalTheories] (theory: EquationalTheory) [HasEquationalTheory theory] (id: Fin theory.ctors.length): Fin BytesCtors.n :=
-  Fin.mk (computeCtorIndex EquationalTheories.theories (HasEquationalTheory.id theory) + (id.val)) (by
-      have := computeCtorIndex_in_bounds EquationalTheories.theories (HasEquationalTheory.id theory) (id.val) (by grind) (by
-        have := HasEquationalTheory.pf theory
-        simp_all
-      )
-      unfold BytesCtors.n instBytesCtorsOfEquationalTheories BytesCtors.ofList
-      assumption
-    )
-
-def EquationalTheory.toGlobalIndex_correct [EquationalTheories] (theory: EquationalTheory) [HasEquationalTheory theory] (id: Fin theory.ctors.length):
-  BytesCtors.ctors (theory.toGlobalIndex id) = theory.ctors[id]
-  := by
-    have := computeCtorIndex_getElem EquationalTheories.theories (HasEquationalTheory.id theory) (id.val) (by grind) (by
-      have := HasEquationalTheory.pf theory
-      simp_all
-    )
-    unfold BytesCtors.ctors instBytesCtorsOfEquationalTheories BytesCtors.ofList EquationalTheory.toGlobalIndex
-    have := HasEquationalTheory.pf theory
-    simp_all
-
-structure EquationalTheories.CtorId [EquationalTheories] where
-  idThy: TheoryId
-  idCtor: Fin (EquationalTheories.theories[idThy].ctors.length)
-
-def fromGlobalIndexAux (l: List EquationalTheory) (id: Nat): Nat × Nat :=
-  match l with
-  | [] => (0, 0) -- unreachable
-  | h::t =>
-    if id < h.ctors.length then (0, id)
-    else
-      let (x, y) := fromGlobalIndexAux t (id - h.ctors.length)
-      (x+1, y)
-
-def fromGlobalIndexAux_in_bounds_1 (l: List EquationalTheory) (id: Nat)
-  (h_id: id < (BytesCtors.ofList (l.flatMap EquationalTheory.ctors)).n)
-  :
-  (fromGlobalIndexAux l id).1 < l.length
-  := by
-    fun_induction fromGlobalIndexAux <;>
-    grind [BytesCtors.n, BytesCtors.ofList]
-
-def fromGlobalIndexAux_in_bounds_2 (l: List EquationalTheory) (id: Nat)
-  (h_id: id < (BytesCtors.ofList (l.flatMap EquationalTheory.ctors)).n)
-  :
-  (fromGlobalIndexAux l id).2 < (l[(fromGlobalIndexAux l id).1]'(fromGlobalIndexAux_in_bounds_1 l id h_id)).ctors.length
-  := by
-    fun_induction fromGlobalIndexAux <;>
-    grind [fromGlobalIndexAux, BytesCtors.n, BytesCtors.ofList]
-
-def fromGlobalIndex [EquationalTheories] (id: CtorId): EquationalTheories.CtorId where
-  idThy := Fin.mk (fromGlobalIndexAux EquationalTheories.theories id).1 (fromGlobalIndexAux_in_bounds_1 EquationalTheories.theories id.val id.isLt)
-  idCtor := Fin.mk (fromGlobalIndexAux EquationalTheories.theories id).2 (fromGlobalIndexAux_in_bounds_2 EquationalTheories.theories id.val id.isLt)
-
-theorem fromGlobalIndexAux_correct
-  (l: List EquationalTheory) (id: Nat)
-  (h_id: id < (BytesCtors.ofList (l.flatMap EquationalTheory.ctors)).n)
-  : (l[(fromGlobalIndexAux l id).1]'(fromGlobalIndexAux_in_bounds_1 l id h_id)).ctors[(fromGlobalIndexAux l id).2]'(fromGlobalIndexAux_in_bounds_2 l id h_id) = (BytesCtors.ofList (l.flatMap EquationalTheory.ctors)).ctors (Fin.mk id h_id)
-  := by
-    fun_induction fromGlobalIndexAux
-    · grind [fromGlobalIndexAux, BytesCtors.n, BytesCtors.ofList]
-    · simp_all [fromGlobalIndexAux, BytesCtors.n, BytesCtors.ofList]
-    · simp only [BytesCtors.ofList, List.flatMap_cons, BytesCtors.n] at h_id
-      simp_all [fromGlobalIndexAux, BytesCtors.n, BytesCtors.ofList]
-      grind
-
-theorem fromGlobalIndex_correct
-  [EquationalTheories]
-  (id: CtorId)
-  : EquationalTheories.theories[(fromGlobalIndex id).idThy].ctors[(fromGlobalIndex id).idCtor] = (BytesCtors.ctors id)
-  := by
-    apply fromGlobalIndexAux_correct EquationalTheories.theories id.val id.isLt
-
-theorem fromGlobalIndexAux_roundtrip
-  (l: List EquationalTheory)
-  (idThy: Nat) (idCtor: Nat)
-  (h_idThy: idThy < l.length)
-  (h_idCtor: idCtor < l[idThy].ctors.length)
-  : (fromGlobalIndexAux l ((computeCtorIndex l idThy) + idCtor)) = (idThy, idCtor)
-  := by
-    fun_induction computeCtorIndex
-    · unfold List.length at h_idThy
-      simp_all
-    · unfold fromGlobalIndexAux
-      grind
-    · simp_all [fromGlobalIndexAux]
-      grind
-
-theorem fromGlobalIndex_roundtrip
-  [EquationalTheories]
-  (idThy: TheoryId) (idCtor: Fin (EquationalTheories.theories[idThy].ctors.length))
-  : (fromGlobalIndex (EquationalTheories.theories[idThy].toGlobalIndex idCtor)) = {idThy, idCtor}
-  := by
-    unfold fromGlobalIndex EquationalTheory.toGlobalIndex
-    have := fromGlobalIndexAux_roundtrip EquationalTheories.theories idThy.val idCtor.val idThy.isLt idCtor.isLt
-    simp_all [HasEquationalTheory.id]
-    obtain ⟨ idCtor, h_idCtor ⟩ := idCtor
-    grind
-
 instance [EquationalTheories] (theory: EquationalTheory) [HasEquationalTheory theory] [theory.CtorsEq ctors]: Bytes.HasCtors ctors where
-  tc id_thy := {
-    id := theory.toGlobalIndex (EquationalTheory.CtorsEq.pf (theory := theory) (ctors := ctors) ▸ id_thy)
-    pf := EquationalTheory.CtorsEq.pf (theory := theory) (ctors := ctors) ▸ theory.toGlobalIndex_correct (EquationalTheory.CtorsEq.pf (theory := theory) (ctors := ctors) ▸ id_thy)
+  tc idCtor := {
+    id := {
+      idThy := HasEquationalTheory.id theory,
+      idCtor := Fin.mk idCtor.val (by simp [HasEquationalTheory.pf theory, EquationalTheory.CtorsEq.pf theory ctors])
+      }
+    pf := by
+      simp [BytesCtors.ctors, HasEquationalTheory.pf theory, EquationalTheory.CtorsEq.pf theory ctors]
   }
+
+-- TODO: is the following useful?
+
+def EquationalTheory.toGlobalIndex
+  [EquationalTheories]
+  (theory: EquationalTheory) [HasEquationalTheory theory]
+  (idCtor: Fin theory.ctors.length)
+  : CtorId
+  where
+    idThy := HasEquationalTheory.id theory
+    idCtor := Fin.mk idCtor.val (by simp [HasEquationalTheory.pf theory])
+
+def EquationalTheory.toGlobalIndex_correct
+  [EquationalTheories]
+  (theory: EquationalTheory) [HasEquationalTheory theory]
+  (id: Fin theory.ctors.length)
+  : BytesCtors.ctors (theory.toGlobalIndex id) = theory.ctors[id]
+  := by
+    simp [BytesCtors.ctors, EquationalTheory.toGlobalIndex, HasEquationalTheory.pf theory]
 
 instance
   [EquationalTheories]
@@ -226,6 +194,6 @@ instance
   (id: Fin theory.ctors.length)
   : theory.ctors[id].HasCtorAt (theory.toGlobalIndex id)
   where
-    pf := theory.toGlobalIndex_correct id
+    pf := by simp [EquationalTheory.toGlobalIndex_correct]
 
 end DY
