DY/Bytes/Invariants.lean
@@ -4,23 +4,26 @@ import DY.Trace
 
 namespace DY
 
+variable {CtorId: Type}
+variable [BytesCtors CtorId]
+
 -- Well formed
 
-def BytesWellFormedT [BytesCtors] := ProofTrace → Prop
-def BytesWellFormedT.default [BytesCtors]: BytesWellFormedT := fun _ => False
+def BytesWellFormedT := ProofTrace → Prop
+def BytesWellFormedT.default: BytesWellFormedT := fun _ => False
 
-class BytesWellFormed [BytesCtors] where
+class BytesWellFormed where
   funs: BytesFunCtors BytesWellFormedT
 
-def Bytes.WellFormed [BytesCtors] [BytesWellFormed] (b: Bytes) : BytesWellFormedT :=
+def Bytes.WellFormed [BytesWellFormed] (b: Bytes) : BytesWellFormedT :=
   Bytes.mkRec BytesWellFormed.funs .default b
 
-class HasBytesWellFormed [BytesCtors] [BytesWellFormed] (id: CtorId) {ctor: BytesCtor} [ctor.HasCtorAt id] (binv: outParam (BytesFunCtor id BytesWellFormedT)) where
+class HasBytesWellFormed [BytesWellFormed] (id: CtorId) {ctor: BytesCtor} [ctor.HasCtorAt id] (binv: outParam (BytesFunCtor id BytesWellFormedT)) where
   pf: BytesWellFormed.funs id = binv.into
   dummy: Unit -- leanprover/lean4#11477 workaround
 
 theorem Bytes.WellFormed.eq
-  [BytesCtors] [tc_binv: BytesWellFormed]
+  [tc_binv: BytesWellFormed]
   (id: CtorId) {ctor: BytesCtor} [ctor.HasCtorAt id]
   {binv: BytesFunCtor id BytesWellFormedT}
   [tc: HasBytesWellFormed id binv]
@@ -37,14 +40,14 @@ grind_pattern Bytes.WellFormed.eq => Bytes.WellFormed (b.pack) tr
 
 -- Well formed later
 
-def BytesWellFormedLaterT [BytesCtors] (bwf: BytesWellFormedT) :=
+def BytesWellFormedLaterT (bwf: BytesWellFormedT) :=
   ∀ tr1 tr2, tr1 ≤ tr2 → bwf tr1 → bwf tr2
 
-class BytesWellFormedLater [BytesCtors] [BytesWellFormed] where
+class BytesWellFormedLater [BytesWellFormed] where
   proofs: BytesFunCtorsProof1 BytesWellFormed.funs BytesWellFormedT.default BytesWellFormedLaterT
 
 theorem Bytes.WellFormed.later
-  [BytesCtors] [BytesWellFormed] [BytesWellFormedLater]
+  [BytesWellFormed] [BytesWellFormedLater]
   (b: Bytes)
   (tr1 tr2: ProofTrace)
   :
@@ -58,32 +61,32 @@ grind_pattern Bytes.WellFormed.later => Bytes.WellFormed b tr1, tr1 ≤ tr2
 
 -- Usage
 
-structure Usage [BytesCtors] where
+structure Usage where
   type: String
   tag: String
   data: Option Bytes
 
-def Usage.nothing [BytesCtors]: Usage where
+def Usage.nothing: Usage where
   type := ""
   tag := ""
   data := none
 
-def GetUsageT [BytesCtors] := ProofTrace → Usage
-def GetUsageT.default [BytesCtors]: GetUsageT := fun _ => Usage.nothing
+def GetUsageT := ProofTrace → Usage
+def GetUsageT.default: GetUsageT := fun _ => Usage.nothing
 
-class GetUsage [BytesCtors] where
+class GetUsage where
   funs: BytesFunCtors GetUsageT
 
 noncomputable
-def Bytes.usage [BytesCtors] [GetUsage] (b: Bytes) : GetUsageT :=
+def Bytes.usage [GetUsage] (b: Bytes) : GetUsageT :=
   Bytes.mkRec GetUsage.funs .default b
 
-class HasGetUsage [BytesCtors] [GetUsage] (id: CtorId) {ctor: BytesCtor} [ctor.HasCtorAt id] (binv: outParam (BytesFunCtor id GetUsageT)) where
+class HasGetUsage [GetUsage] (id: CtorId) {ctor: BytesCtor} [ctor.HasCtorAt id] (binv: outParam (BytesFunCtor id GetUsageT)) where
   pf: GetUsage.funs id = binv.into
   dummy: Unit -- leanprover/lean4#11477 workaround
 
 theorem Bytes.usage.eq
-  [BytesCtors] [tc_binv: GetUsage]
+  [tc_binv: GetUsage]
   (id: CtorId) {ctor: BytesCtor} [ctor.HasCtorAt id]
   {binv: BytesFunCtor id GetUsageT}
   [tc: HasGetUsage id binv]
@@ -100,15 +103,15 @@ grind_pattern Bytes.usage.eq => Bytes.usage (b.pack) tr
 
 -- Usage later
 
-def GetUsageLaterT [BytesCtors] (x: BytesWellFormedT × GetUsageT) :=
+def GetUsageLaterT (x: BytesWellFormedT × GetUsageT) :=
   let (wf, usg) := x
   ∀ tr1 tr2: ProofTrace, tr1 ≤ tr2 → wf tr1 → usg tr1 = usg tr2
 
-class GetUsageLater [BytesCtors] [BytesWellFormed] [GetUsage] where
+class GetUsageLater [BytesWellFormed] [GetUsage] where
   proofs: BytesFunCtorsProof2 BytesWellFormed.funs GetUsage.funs BytesWellFormedT.default GetUsageT.default GetUsageLaterT
 
 theorem Bytes.usage_later
-  [BytesCtors] [BytesWellFormed] [GetUsage] [GetUsageLater]
+  [BytesWellFormed] [GetUsage] [GetUsageLater]
   (b: Bytes)
   (tr1 tr2: ProofTrace)
   :
@@ -122,22 +125,22 @@ grind_pattern Bytes.usage_later => Bytes.usage b tr1, tr1 ≤ tr2
 
 -- Label
 
-def GetLabelT [BytesCtors] := ProofTrace → Label
-def GetLabelT.default [BytesCtors]: GetLabelT := fun _ => Label.secret
+def GetLabelT := ProofTrace → Label
+def GetLabelT.default: GetLabelT := fun _ => Label.secret
 
-class GetLabel [BytesCtors] where
+class GetLabel where
   funs: BytesFunCtors GetLabelT
 
 noncomputable
-def Bytes.label [BytesCtors] [GetLabel] (b: Bytes) : GetLabelT :=
+def Bytes.label [GetLabel] (b: Bytes) : GetLabelT :=
   Bytes.mkRec GetLabel.funs .default b
 
-class HasGetLabel [BytesCtors] [GetLabel] (id: CtorId) {ctor: BytesCtor} [ctor.HasCtorAt id] (binv: outParam (BytesFunCtor id GetLabelT)) where
+class HasGetLabel [GetLabel] (id: CtorId) {ctor: BytesCtor} [ctor.HasCtorAt id] (binv: outParam (BytesFunCtor id GetLabelT)) where
   pf: GetLabel.funs id = binv.into
   dummy: Unit -- leanprover/lean4#11477 workaround
 
 theorem Bytes.label.eq
-  [BytesCtors] [tc_binv: GetLabel]
+  [tc_binv: GetLabel]
   (id: CtorId) {ctor: BytesCtor} [ctor.HasCtorAt id]
   {binv: BytesFunCtor id GetLabelT}
   [tc: HasGetLabel id binv]
@@ -154,15 +157,15 @@ grind_pattern Bytes.label.eq => Bytes.label (b.pack) tr
 
 -- Label later
 
-def GetLabelLaterT [BytesCtors] (x: BytesWellFormedT × GetLabelT) :=
+def GetLabelLaterT (x: BytesWellFormedT × GetLabelT) :=
   let (wf, usg) := x
   ∀ tr1 tr2: ProofTrace, tr1 ≤ tr2 → wf tr1 → usg tr1 = usg tr2
 
-class GetLabelLater [BytesCtors] [BytesWellFormed] [GetLabel] where
+class GetLabelLater [BytesWellFormed] [GetLabel] where
   proofs: BytesFunCtorsProof2 BytesWellFormed.funs GetLabel.funs BytesWellFormedT.default GetLabelT.default GetLabelLaterT
 
 theorem Bytes.label_later
-  [BytesCtors] [BytesWellFormed] [GetLabel] [GetLabelLater]
+  [BytesWellFormed] [GetLabel] [GetLabelLater]
   (b: Bytes)
   (tr1 tr2: ProofTrace)
   :
@@ -176,22 +179,22 @@ grind_pattern Bytes.label_later => Bytes.label b tr1, tr1 ≤ tr2
 
 -- Invariant
 
-def BytesInvariantT [BytesCtors] := ProofTrace → Prop
+def BytesInvariantT := ProofTrace → Prop
 
-def BytesInvariantT.default [BytesCtors]: BytesInvariantT := fun _ => False
+def BytesInvariantT.default: BytesInvariantT := fun _ => False
 
-class BytesInvariant [BytesCtors] where
+class BytesInvariant where
   funs: BytesFunCtors BytesInvariantT
 
-def Bytes.Invariant [BytesCtors] [BytesInvariant] (b: Bytes) (tr: ProofTrace) : Prop :=
+def Bytes.Invariant [BytesInvariant] (b: Bytes) (tr: ProofTrace) : Prop :=
   Bytes.mkRec BytesInvariant.funs .default b tr
 
-class HasBytesInvariant [BytesCtors] [BytesInvariant] (id: CtorId) {ctor: BytesCtor} [ctor.HasCtorAt id] (binv: outParam (BytesFunCtor id BytesInvariantT)) where
+class HasBytesInvariant [BytesInvariant] (id: CtorId) {ctor: BytesCtor} [ctor.HasCtorAt id] (binv: outParam (BytesFunCtor id BytesInvariantT)) where
   pf: BytesInvariant.funs id = binv.into
   dummy: Unit -- leanprover/lean4#11477 workaround
 
 theorem Bytes.Invariant.eq
-  [BytesCtors] [tc_binv: BytesInvariant]
+  [tc_binv: BytesInvariant]
   (id: CtorId) {ctor: BytesCtor} [ctor.HasCtorAt id]
   {binv: BytesFunCtor id BytesInvariantT}
   [tc: HasBytesInvariant id binv]
@@ -208,15 +211,15 @@ grind_pattern Bytes.Invariant.eq => Bytes.Invariant (b.pack) tr
 
 -- Invariant implies well formed
 
-def BytesInvariantImpliesBytesWellFormedT [BytesCtors] (x: BytesInvariantT × BytesWellFormedT) :=
+def BytesInvariantImpliesBytesWellFormedT (x: BytesInvariantT × BytesWellFormedT) :=
   let (binv, bwf) := x
   ∀ tr, binv tr → bwf tr
 
-class BytesInvariantImpliesBytesWellFormed [BytesCtors] [BytesWellFormed] [BytesInvariant] where
+class BytesInvariantImpliesBytesWellFormed [BytesWellFormed] [BytesInvariant] where
   proofs: BytesFunCtorsProof2 BytesInvariant.funs BytesWellFormed.funs BytesInvariantT.default BytesWellFormedT.default BytesInvariantImpliesBytesWellFormedT
 
 theorem Bytes.Invariant_implies_WellFormed
-  [BytesCtors] [BytesWellFormed] [BytesInvariant] [BytesInvariantImpliesBytesWellFormed]
+  [BytesWellFormed] [BytesInvariant] [BytesInvariantImpliesBytesWellFormed]
   (b: Bytes)
   (tr: ProofTrace)
   :
@@ -229,14 +232,14 @@ grind_pattern Bytes.Invariant_implies_WellFormed => Bytes.WellFormed b tr
 
 -- Invariant later
 
-def BytesInvariantLaterT [BytesCtors] (binv: BytesInvariantT) :=
+def BytesInvariantLaterT (binv: BytesInvariantT) :=
   ∀ tr1 tr2, tr1 ≤ tr2 → binv tr1 → binv tr2
 
-class BytesInvariantLater [BytesCtors] [BytesInvariant] where
+class BytesInvariantLater [BytesInvariant] where
   proofs: BytesFunCtorsProof1 BytesInvariant.funs BytesInvariantT.default BytesInvariantLaterT
 
 theorem Bytes.Invariant.later
-  [BytesCtors] [BytesInvariant] [BytesInvariantLater]
+  [BytesInvariant] [BytesInvariantLater]
   (b: Bytes)
   (tr1 tr2: ProofTrace)
   :
@@ -248,7 +251,7 @@ theorem Bytes.Invariant.later
 
 grind_pattern Bytes.Invariant.later => Bytes.Invariant b tr1, tr1 ≤ tr2
 
-structure BytesCtorInvariants.Internal [BytesCtors] (ctor: BytesCtor) where
+structure BytesCtorInvariants.Internal (ctor: BytesCtor) where
   well_formed: BytesFunCtor.Internal ctor BytesWellFormedT
   well_formed_later: [BytesWellFormed] → BytesFunCtorProof1.Internal Bytes.WellFormed well_formed BytesWellFormedLaterT
 
@@ -263,11 +266,11 @@ structure BytesCtorInvariants.Internal [BytesCtors] (ctor: BytesCtor) where
   invariant_later: [BytesWellFormed] → [BytesWellFormedLater] → [GetUsage] → [GetUsageLater] → [GetLabel] → [GetLabelLater] → [BytesInvariant] → [BytesInvariantImpliesBytesWellFormed] → BytesFunCtorProof1.Internal Bytes.Invariant invariant BytesInvariantLaterT
   -- ...
 
-def BytesCtorInvariants.ById [BytesCtors] (id: CtorId) := BytesCtorInvariants.Internal (BytesCtors.ctors id)
-def BytesCtorInvariants [BytesCtors] (id: CtorId) {ctor: BytesCtor} [ctor.HasCtorAt id] := BytesCtorInvariants.Internal ctor
+def BytesCtorInvariants.ById (id: CtorId) := BytesCtorInvariants.Internal (BytesCtors.ctors id)
+def BytesCtorInvariants (id: CtorId) {ctor: BytesCtor} [ctor.HasCtorAt id] := BytesCtorInvariants.Internal ctor
 
 def BytesCtorInvariants.into
-  [BytesCtors] {id: CtorId} {ctor: BytesCtor} [ctor.HasCtorAt id]
+  {id: CtorId} {ctor: BytesCtor} [ctor.HasCtorAt id]
   (f: BytesCtorInvariants id)
   : BytesCtorInvariants.ById id
   where
@@ -285,66 +288,66 @@ def BytesCtorInvariants.into
     invariant_later := BytesFunCtorProof1.into f.invariant_later
 
 
-class BytesCtorsInvariants [BytesCtors] where
+class BytesCtorsInvariants where
   funs: (id: CtorId) → BytesCtorInvariants.ById id
 
-instance [BytesCtors] [BytesCtorsInvariants]: BytesWellFormed where
+instance [BytesCtorsInvariants]: BytesWellFormed where
   funs id := (BytesCtorsInvariants.funs id).well_formed
 
-instance [BytesCtors] [BytesCtorsInvariants]: BytesWellFormedLater where
+instance [BytesCtorsInvariants]: BytesWellFormedLater where
   proofs id := (BytesCtorsInvariants.funs id).well_formed_later
 
-instance [BytesCtors] [BytesCtorsInvariants]: GetUsage where
+instance [BytesCtorsInvariants]: GetUsage where
   funs id := (BytesCtorsInvariants.funs id).usage
 
-instance [BytesCtors] [BytesCtorsInvariants]: GetUsageLater where
+instance [BytesCtorsInvariants]: GetUsageLater where
   proofs id := (BytesCtorsInvariants.funs id).usage_later
 
-instance [BytesCtors] [BytesCtorsInvariants]: GetLabel where
+instance [BytesCtorsInvariants]: GetLabel where
   funs id := (BytesCtorsInvariants.funs id).label
 
-instance [BytesCtors] [BytesCtorsInvariants]: GetLabelLater where
+instance [BytesCtorsInvariants]: GetLabelLater where
   proofs id := (BytesCtorsInvariants.funs id).label_later
 
-instance [BytesCtors] [BytesCtorsInvariants]: BytesInvariant where
+instance [BytesCtorsInvariants]: BytesInvariant where
   funs id := (BytesCtorsInvariants.funs id).invariant
 
-instance [BytesCtors] [BytesCtorsInvariants]: BytesInvariantImpliesBytesWellFormed where
+instance [BytesCtorsInvariants]: BytesInvariantImpliesBytesWellFormed where
   proofs id := (BytesCtorsInvariants.funs id).invariant_implies_wellformed
 
-instance [BytesCtors] [BytesCtorsInvariants]: BytesInvariantLater where
+instance [BytesCtorsInvariants]: BytesInvariantLater where
   proofs id := (BytesCtorsInvariants.funs id).invariant_later
 
-class HasBytesInvariants [BytesCtors] [BytesCtorsInvariants] (id: CtorId) {ctor: BytesCtor} [ctor.HasCtorAt id] (funs: outParam (BytesCtorInvariants id)) where
+class HasBytesInvariants [BytesCtorsInvariants] (id: CtorId) {ctor: BytesCtor} [ctor.HasCtorAt id] (funs: outParam (BytesCtorInvariants id)) where
   pf: BytesCtorsInvariants.funs id = funs.into
 
-instance [BytesCtors] [BytesCtorsInvariants] (id: CtorId) {ctor: BytesCtor} [ctor.HasCtorAt id] (funs: BytesCtorInvariants id) [tc: HasBytesInvariants id funs]: HasBytesWellFormed id funs.well_formed where
+instance [BytesCtorsInvariants] (id: CtorId) {ctor: BytesCtor} [ctor.HasCtorAt id] (funs: BytesCtorInvariants id) [tc: HasBytesInvariants id funs]: HasBytesWellFormed id funs.well_formed where
   pf := by simp only [BytesWellFormed.funs, tc.pf, BytesCtorInvariants.into]
   dummy := ()
 
-instance [BytesCtors] [BytesCtorsInvariants] (id: CtorId) {ctor: BytesCtor} [ctor.HasCtorAt id] (funs: BytesCtorInvariants id) [tc: HasBytesInvariants id funs]: HasGetUsage id funs.usage where
+instance [BytesCtorsInvariants] (id: CtorId) {ctor: BytesCtor} [ctor.HasCtorAt id] (funs: BytesCtorInvariants id) [tc: HasBytesInvariants id funs]: HasGetUsage id funs.usage where
   pf := by simp only [GetUsage.funs, tc.pf, BytesCtorInvariants.into]
   dummy := ()
 
-instance [BytesCtors] [BytesCtorsInvariants] (id: CtorId) {ctor: BytesCtor} [ctor.HasCtorAt id] (funs: BytesCtorInvariants id) [tc: HasBytesInvariants id funs]: HasGetLabel id funs.label where
+instance [BytesCtorsInvariants] (id: CtorId) {ctor: BytesCtor} [ctor.HasCtorAt id] (funs: BytesCtorInvariants id) [tc: HasBytesInvariants id funs]: HasGetLabel id funs.label where
   pf := by simp only [GetLabel.funs, tc.pf, BytesCtorInvariants.into]
   dummy := ()
 
-instance [BytesCtors] [BytesCtorsInvariants] (id: CtorId) {ctor: BytesCtor} [ctor.HasCtorAt id] (funs: BytesCtorInvariants id) [tc: HasBytesInvariants id funs]: HasBytesInvariant id funs.invariant where
+instance [BytesCtorsInvariants] (id: CtorId) {ctor: BytesCtor} [ctor.HasCtorAt id] (funs: BytesCtorInvariants id) [tc: HasBytesInvariants id funs]: HasBytesInvariant id funs.invariant where
   pf := by simp only [BytesInvariant.funs, tc.pf, BytesCtorInvariants.into]
   dummy := ()
 
 @[grind]
-def Bytes.Publishable [BytesCtors] [BytesCtorsInvariants] (b: Bytes) (tr: ProofTrace) :=
+def Bytes.Publishable [BytesCtorsInvariants] (b: Bytes) (tr: ProofTrace) :=
   b.Invariant tr ∧
   (b.label tr).canFlow Label.pub tr
 
-def Bytes.HasUsage [BytesCtors] [GetUsage] [GetLabel] (b: Bytes) (usg: Usage) (tr: ProofTrace) :=
+def Bytes.HasUsage [GetUsage] [GetLabel] (b: Bytes) (usg: Usage) (tr: ProofTrace) :=
   b.usage tr = usg ∨
   (b.label tr).canFlow Label.pub tr
 
 theorem Bytes.HasUsage_later
-  [BytesCtors] [BytesWellFormed] [GetUsage] [GetUsageLater] [GetLabel] [GetLabelLater]
+  [BytesWellFormed] [GetUsage] [GetUsageLater] [GetLabel] [GetLabelLater]
   (b: Bytes) (usg: Usage) (tr1 tr2: ProofTrace)
   :
     b.WellFormed tr1 →
@@ -357,7 +360,7 @@ theorem Bytes.HasUsage_later
 grind_pattern Bytes.HasUsage_later => b.HasUsage usg tr1, tr1 ≤ tr2
 
 theorem Bytes.HasUsage_inj
-  [BytesCtors] [BytesWellFormed] [GetUsage] [GetUsageLater] [GetLabel] [GetLabelLater]
+  [BytesWellFormed] [GetUsage] [GetUsageLater] [GetLabel] [GetLabelLater]
   (b: Bytes) (usg1 usg2: Usage) (tr: ProofTrace)
   :
     b.HasUsage usg1 tr →
@@ -367,7 +370,7 @@ theorem Bytes.HasUsage_inj
     grind [Bytes.HasUsage]
 
 theorem Bytes.HasUsage_public
-  [BytesCtors] [BytesWellFormed] [GetUsage] [GetUsageLater] [GetLabel] [GetLabelLater]
+  [BytesWellFormed] [GetUsage] [GetUsageLater] [GetLabel] [GetLabelLater]
   (b: Bytes) (usg: Usage) (tr: ProofTrace)
   :
     (b.label tr).canFlow Label.pub tr →
@@ -377,7 +380,7 @@ theorem Bytes.HasUsage_public
 
 noncomputable
 def Bytes.xxxLabel
-  [BytesCtors] [GetLabel]
+  [GetLabel]
   (extract: Bytes → Option Bytes)
   (b: Bytes) (tr: ProofTrace) :=
     match extract b with
@@ -385,14 +388,14 @@ def Bytes.xxxLabel
     | none => Label.pub
 
 def Bytes.XXXHasUsage
-  [BytesCtors] [GetUsage] [GetLabel]
+  [GetUsage] [GetLabel]
   (extract: Bytes → Option Bytes)
   (b: Bytes) (usg: Usage) (tr: ProofTrace) :=
     match extract b with
     | some sk => sk.HasUsage usg tr
     | none => True
 
-def ExtractPreservesWellFormed [BytesCtors] [BytesWellFormed] (extract: Bytes → Option Bytes): Prop :=
+def ExtractPreservesWellFormed [BytesWellFormed] (extract: Bytes → Option Bytes): Prop :=
   ∀ b tr, b.WellFormed tr → (
     match extract b with
     | some b' => b'.WellFormed tr
@@ -400,7 +403,7 @@ def ExtractPreservesWellFormed [BytesCtors] [BytesWellFormed] (extract: Bytes �
   )
 
 theorem Bytes.xxxLabel_later
-  [BytesCtors] [BytesWellFormed] [GetLabel] [GetLabelLater]
+  [BytesWellFormed] [GetLabel] [GetLabelLater]
   (extract: Bytes → Option Bytes)
   (h_extract: ExtractPreservesWellFormed extract)
   (b: Bytes) (tr1 tr2: ProofTrace)
@@ -413,7 +416,7 @@ theorem Bytes.xxxLabel_later
     grind [ExtractPreservesWellFormed]
 
 theorem Bytes.XXXHasUsage_later
-  [BytesCtors] [BytesWellFormed] [GetUsage] [GetUsageLater] [GetLabel] [GetLabelLater]
+  [BytesWellFormed] [GetUsage] [GetUsageLater] [GetLabel] [GetLabelLater]
   (extract: Bytes → Option Bytes)
   (h_extract: ExtractPreservesWellFormed extract)
   (b: Bytes) (usg: Usage) (tr1 tr2: ProofTrace)
