DY/SignedDH.lean
@@ -333,9 +333,9 @@ where
 def signMetaprog: GhostParameterFinder where
   findGhost mvar e :=
   Lean.withTraceNode `Step (fun _ => pure m!"signMetaprog") do
-    let sk_mvar ← Lean.Meta.mkFreshExprMVar (some (← Lean.Meta.mkAppOptM ``Bytes #[none]))
-    let nonce_mvar ← Lean.Meta.mkFreshExprMVar (some (← Lean.Meta.mkAppOptM ``Bytes #[none]))
-    let msg_mvar ← Lean.Meta.mkFreshExprMVar (some (← Lean.Meta.mkAppOptM ``Bytes #[none]))
+    let sk_mvar ← Lean.Meta.mkFreshExprMVar (some (← Lean.Meta.mkAppOptM ``Bytes #[none, none]))
+    let nonce_mvar ← Lean.Meta.mkFreshExprMVar (some (← Lean.Meta.mkAppOptM ``Bytes #[none, none]))
+    let msg_mvar ← Lean.Meta.mkFreshExprMVar (some (← Lean.Meta.mkAppOptM ``Bytes #[none, none]))
     let signToUnify ← Lean.Meta.mkAppM ``Signature.sign #[sk_mvar, nonce_mvar, msg_mvar]
     trace[Step] "gonna unify {e} and {signToUnify}"
     unless ← Lean.Meta.isDefEq e signToUnify do
@@ -343,8 +343,8 @@ def signMetaprog: GhostParameterFinder where
     trace[Step] "got {signToUnify}"
 
     let usg_mvar: Lean.Expr := .mvar mvar
-    let tr_mvar ← Lean.Meta.mkFreshExprMVar (some (← Lean.Meta.mkAppOptM ``ProofTrace #[none]))
-    let hasUsageToUnify ← Lean.Meta.mkAppOptM ``Bytes.HasUsage #[none, none, none, sk_mvar, usg_mvar, tr_mvar]
+    let tr_mvar ← Lean.Meta.mkFreshExprMVar (some (← Lean.Meta.mkAppOptM ``ProofTrace #[none, none]))
+    let hasUsageToUnify ← Lean.Meta.mkAppOptM ``Bytes.HasUsage #[none, none, none, none, sk_mvar, usg_mvar, tr_mvar]
     trace[Step] "gonna find {hasUsageToUnify} in assumptions"
     let .mvar hasUsageMvar ← Lean.Meta.mkFreshExprMVar hasUsageToUnify
       | throwError ""
@@ -392,9 +392,9 @@ where
 def verifyMetaprog: GhostParameterFinder where
   findGhost mvar e :=
   Lean.withTraceNode `Step (fun _ => pure m!"verifyMetaprog") do
-    let vkey_mvar ← Lean.Meta.mkFreshExprMVar (some (← Lean.Meta.mkAppOptM ``Bytes #[none]))
-    let msg_mvar ← Lean.Meta.mkFreshExprMVar (some (← Lean.Meta.mkAppOptM ``Bytes #[none]))
-    let sig_mvar ← Lean.Meta.mkFreshExprMVar (some (← Lean.Meta.mkAppOptM ``Bytes #[none]))
+    let vkey_mvar ← Lean.Meta.mkFreshExprMVar (some (← Lean.Meta.mkAppOptM ``Bytes #[none, none]))
+    let msg_mvar ← Lean.Meta.mkFreshExprMVar (some (← Lean.Meta.mkAppOptM ``Bytes #[none, none]))
+    let sig_mvar ← Lean.Meta.mkFreshExprMVar (some (← Lean.Meta.mkAppOptM ``Bytes #[none, none]))
     let verifyToUnify ← Lean.Meta.mkAppM ``Signature.verify #[vkey_mvar, msg_mvar, sig_mvar]
     trace[Step] "gonna unify {e} and {verifyToUnify}"
     unless ← Lean.Meta.isDefEq e verifyToUnify do
@@ -402,7 +402,7 @@ def verifyMetaprog: GhostParameterFinder where
     trace[Step] "got {verifyToUnify}"
 
     let usg_mvar: Lean.Expr := .mvar mvar
-    let tr_mvar ← Lean.Meta.mkFreshExprMVar (some (← Lean.Meta.mkAppOptM ``ProofTrace #[none]))
+    let tr_mvar ← Lean.Meta.mkFreshExprMVar (some (← Lean.Meta.mkAppOptM ``ProofTrace #[none, none]))
     let hasUsageToUnify ← Lean.Meta.mkAppOptM ``Bytes.SignkeyHasUsage #[none, none, none, none, vkey_mvar, usg_mvar, tr_mvar]
     trace[Step] "gonna find {hasUsageToUnify} in assumptions"
     let .mvar hasUsageMvar ← Lean.Meta.mkFreshExprMVar hasUsageToUnify
